update enc_cipher_ok for growing key heaps
To accommodate key generation, we need to show that encrypted_cipher_ok
is preserved by the addition of another honest key. This requires that
the key is *actually* new, i.e. that it could not have been used to
sign/encrypt a cipher previously blessed by encrypted_cipher_ok.

We therefore include the global key heap as a parameter to
encrypted_cipher_ok and stipulate in its constructors that:
1) the signing/encryption keys must be in the global key heap
2) any (private) keys in the message to be packaged must be in the
global key heap.

Then to show preservation, we need only know that the new key was not
previously in the global key heap (a fact which follows directly from
the key generation steps in the operational semantics).

I've also included some automation which may or may not have application
in other proofs where key_perm manipulation is required.

KeyManagement/Simulation.v
@@ -106,29 +106,57 @@ Section RealWorldUniverseProperties.
     Forall_natmap
       (fun u => user_cipher_queue_ok cs honestk u.(c_heap)) usrs.
 
-  Inductive encrypted_cipher_ok (cs : ciphers) : cipher -> Prop :=
-  | SigCipherHonestOk : forall {t} (msg : message t) k,
+  (* Inductive encrypted_cipher_ok (cs : ciphers) : cipher -> Prop := *)
+  (* | SigCipherHonestOk : forall {t} (msg : message t) k, *)
+  (*     honestk $? k = Some true *)
+  (*     -> (forall k, findKeys msg $? k = Some true -> False) *)
+  (*     -> msgCiphersSigned honestk cs msg *)
+  (*     -> encrypted_cipher_ok cs (SigCipher k msg) *)
+  (* | SigCipherNotHonestOk : forall {t} (msg : message t) k, *)
+  (*     honestk $? k <> Some true *)
+  (*     -> encrypted_cipher_ok cs (SigCipher k msg) *)
+  (* | SigEncCipherAdvSignedOk :  forall {t} (msg : message t) k__e k__s, *)
+  (*     honestk $? k__s <> Some true *)
+  (*     -> (forall k, findKeys msg $? k = Some true *)
+  (*             -> honestk $? k <> Some true) *)
+  (*     -> encrypted_cipher_ok cs (SigEncCipher k__s k__e msg) *)
+  (* | SigEncCipherHonestSignedEncKeyHonestOk : forall {t} (msg : message t) k__e k__s, *)
+  (*     honestk $? k__s = Some true *)
+  (*     -> honestk $? k__e = Some true *)
+  (*     -> keys_mine honestk (findKeys msg) *)
+  (*     -> msgCiphersSigned honestk cs msg *)
+  (*     -> encrypted_cipher_ok cs (SigEncCipher k__s k__e msg). *)
+
+  Inductive encrypted_cipher_ok (cs : ciphers) (gks : keys): cipher -> Prop :=
+  | SigCipherHonestOk : forall {t} (msg : message t) k k_data,
       honestk $? k = Some true
+      -> gks $? k = Some k_data
       -> (forall k, findKeys msg $? k = Some true -> False)
       -> msgCiphersSigned honestk cs msg
-      -> encrypted_cipher_ok cs (SigCipher k msg)
-  | SigCipherNotHonestOk : forall {t} (msg : message t) k,
+      -> encrypted_cipher_ok cs gks (SigCipher k msg)
+  | SigCipherNotHonestOk : forall {t} (msg : message t) k k_data,
       honestk $? k <> Some true
-      -> encrypted_cipher_ok cs (SigCipher k msg)
-  | SigEncCipherAdvSignedOk :  forall {t} (msg : message t) k__e k__s,
+      -> gks $? k = Some k_data
+      -> encrypted_cipher_ok cs gks (SigCipher k msg)
+  | SigEncCipherAdvSignedOk :  forall {t} (msg : message t) k__s k__e k_data__s k_data__e,
       honestk $? k__s <> Some true
+      -> gks $? k__s = Some k_data__s
+      -> gks $? k__e = Some k_data__e
       -> (forall k, findKeys msg $? k = Some true
-              -> honestk $? k <> Some true)
-      -> encrypted_cipher_ok cs (SigEncCipher k__s k__e msg)
-  | SigEncCipherHonestSignedEncKeyHonestOk : forall {t} (msg : message t) k__e k__s,
+              -> exists v, gks $? k = Some v
+                     /\ honestk $? k <> Some true)
+      -> encrypted_cipher_ok cs gks (SigEncCipher k__s k__e msg)
+  | SigEncCipherHonestSignedEncKeyHonestOk : forall {t} (msg : message t) k__s k__e k_data__s k_data__e,
       honestk $? k__s = Some true
       -> honestk $? k__e = Some true
+      -> gks $? k__s = Some k_data__s
+      -> gks $? k__e = Some k_data__e
       -> keys_mine honestk (findKeys msg)
       -> msgCiphersSigned honestk cs msg
-      -> encrypted_cipher_ok cs (SigEncCipher k__s k__e msg).
+      -> encrypted_cipher_ok cs gks (SigEncCipher k__s k__e msg).
 
-  Definition encrypted_ciphers_ok (cs : ciphers) :=
-    Forall_natmap (encrypted_cipher_ok cs) cs.
+  Definition encrypted_ciphers_ok (cs : ciphers) (gks : keys) :=
+    Forall_natmap (encrypted_cipher_ok cs gks) cs.
 
   Definition message_no_adv_private {t} (msg : message t) :=
     forall k, findKeys msg $? k = Some true -> False.
@@ -179,7 +207,7 @@ End RealWorldUniverseProperties.
 
 Definition universe_ok {A B} (U : RealWorld.universe A B) : Prop :=
   let honestk := RealWorld.findUserKeys U.(RealWorld.users)
-  in  encrypted_ciphers_ok honestk U.(RealWorld.all_ciphers)
+  in  encrypted_ciphers_ok honestk U.(RealWorld.all_ciphers) U.(RealWorld.all_keys)
 .
 
 Definition adv_universe_ok {A B} (U : RealWorld.universe A B) : Prop :=
@@ -276,10 +304,10 @@ Proof.
 Qed.
 
 Lemma encrypted_cipher_ok_addnl_cipher :
-  forall honestk cs c_id c1 c2,
-    encrypted_cipher_ok honestk cs c1
+  forall honestk cs gks c_id c1 c2,
+    encrypted_cipher_ok honestk cs gks c1
     -> ~ In c_id cs
-    -> encrypted_cipher_ok honestk (cs $+ (c_id,c2)) c1.
+    -> encrypted_cipher_ok honestk (cs $+ (c_id,c2)) gks c1.
 Proof.
   inversion 1; intros; try solve [ econstructor; eauto ].
   - econstructor; eauto.
@@ -289,10 +317,10 @@ Proof.
 Qed.
 
 Lemma encrypted_ciphers_ok_addnl_cipher :
-  forall honestk cs c_id c,
-    Forall_natmap (encrypted_cipher_ok honestk cs) cs
+  forall honestk cs gks c_id c,
+    Forall_natmap (encrypted_cipher_ok honestk cs gks) cs
     -> ~ In c_id cs
-    -> Forall_natmap (encrypted_cipher_ok honestk (cs $+ (c_id, c))) cs.
+    -> Forall_natmap (encrypted_cipher_ok honestk (cs $+ (c_id, c)) gks) cs.
 Proof.
   intros.
   rewrite Forall_natmap_forall in *.
@@ -300,3 +328,82 @@ Proof.
   specialize (H _ _ H1); eauto using encrypted_cipher_ok_addnl_cipher.
 Qed.
 
+Ltac solve_against_key k k' := destruct (k ==n k'); subst; clean_map_lookups; eauto.
+
+Ltac add_key_solver' honestk k_id k' :=
+      unfold add_key_perm; destruct (honestk $? k_id); simplify; eauto; solve_against_key k_id k'.
+
+Ltac add_key_solver :=
+  match goal with
+  | [|- _ $+ (?k_id, _) $? ?k' = _] => solve_against_key k_id k'
+  | [|- context[_ $? ?k']] =>
+    match goal with
+    | [|- context[add_key_perm ?k_id _ ?honestk]] => add_key_solver' honestk k_id k'
+    | [|- context[?honestk $+ (?k_id, _)]] => add_key_solver' honestk k_id k'
+    end
+  end.
+
+Lemma messageCipherOk_addnl_key : forall honestk cs msg k_id,
+    RealWorld.msgCipherOk honestk cs msg
+    -> RealWorld.msgCipherOk (add_key_perm k_id true honestk) cs msg.
+Proof.
+  intros.
+  unfold RealWorld.msgCipherOk in *.
+  destruct msg.
+  intuition idtac.
+  destruct m
+  ; eauto
+  ; unfold RealWorld.msg_honestly_signed, RealWorld.honest_keyb in *
+  ; add_key_solver.
+Qed.
+
+Lemma keys_mine_addnl_key : forall {t} honestk k_id (msg : RealWorld.message t),
+  RealWorld.keys_mine honestk (RealWorld.findKeys msg)
+  -> RealWorld.keys_mine (add_key_perm k_id true honestk) (RealWorld.findKeys msg).
+  unfold RealWorld.keys_mine in *; intros; destruct kp; add_key_solver.
+Qed.
+
+Lemma dishonest_sigenc_addnl_key : forall {t} honestk k_id k_data (gks : keys) (msg : RealWorld.message t),
+    (forall k, RealWorld.findKeys msg $? k = Some true
+          -> exists v, gks $? k = Some v
+                 /\ honestk $? k <> Some true)
+    -> gks $? k_id = None
+    -> (forall k, RealWorld.findKeys msg $? k = Some true
+            -> exists v, gks $+ (k_id, k_data) $? k = Some v
+                   /\ (add_key_perm k_id true honestk) $? k <> Some true).
+  intros.
+  apply H in H1 as [v [J K]].
+  add_key_solver.
+Qed.
+
+Hint Resolve messageCipherOk_addnl_key keys_mine_addnl_key dishonest_sigenc_addnl_key.
+
+Lemma msgCiphersSigned_addnl_key : forall {t} honestk cs (msg : RealWorld.message t) k_id,
+    RealWorld.msgCiphersSigned honestk cs msg
+    -> RealWorld.msgCiphersSigned (add_key_perm k_id true honestk) cs msg.
+Proof.
+  intros; invert H; unfold RealWorld.msgCiphersSigned in *.
+  - rewrite <- H1. constructor.
+  - apply Forall_forall.
+    intros.
+    rewrite Forall_forall in H2.
+    rewrite <- H0 in H.
+    destruct H; subst; auto.
+Qed.
+
+Hint Resolve msgCiphersSigned_addnl_key.
+
+Lemma encrypted_cipher_ok_addnl_key :
+  forall honestk cs gks c_id k_id k_data,
+    encrypted_cipher_ok honestk cs gks c_id
+    -> gks $? k_id = None
+    -> encrypted_cipher_ok (add_key_perm k_id true honestk) cs (gks $+ (k_id, k_data)) c_id.
+Proof.
+  intros
+  ; invert H
+  ; [ eapply SigCipherHonestOk
+    | eapply SigCipherNotHonestOk
+    | eapply SigEncCipherAdvSignedOk
+    | eapply SigEncCipherHonestSignedEncKeyHonestOk]
+  ; (eauto || add_key_solver).
+Qed.
